Proofs: definition of ctx_hdn_shift of type ctx

ott_coq/destination_calculus_ott.v
@@ -6,6 +6,7 @@ Require Import List.
 Require Import Ott.ott_list_core.
 
 
+Import EqNotations.
 Require Import Ott.ext_nat.
 Require Import Coq.Structures.Equalities.
 Require Import Coq.Arith.PeanoNat.
@@ -13,6 +14,7 @@ Require Import Coq.Arith.Compare_dec.
 Require Import Coq.MSets.MSetList.
 Require Import Coq.MSets.MSetFacts.
 Require List.
+Require Import Coq.Logic.FunctionalExtensionality.
 (* Grumble, grumble: we shouldn't need to Import Ott.Finitely, but if
    we don't we can't use the coercions. *)
 Require Import Ott.Finitely.
@@ -117,16 +119,16 @@ Inductive type : Type :=  (*r Type *)
  | type_F (T:type) (m:mode) (U:type) (*r Function *)
  | type_D (T:type) (m:mode) (*r Destination *).
 
-Inductive name : Type := 
+Inductive name : Type :=
  | name_Var (x:var)
  | name_DH (h:hdn).
 
 Definition ectxs : Type := (list ectx).
 
-Inductive tyb_var : Type := 
+Inductive tyb_var : Type :=
  | tyb_Var (m:mode) (T:type).
 
-Inductive tyb_dh : Type := 
+Inductive tyb_dh : Type :=
  | tyb_Dest (m:mode) (T:type) (n:mode)
  | tyb_Hole (T:type) (n:mode).
 Lemma eq_type: forall (x y : type), {x = y} + {x <> y}.
@@ -219,7 +221,7 @@ Fixpoint term_sub (te: term) (x':var) (v':val) : term := match te with
   | term_PatP t m x1 x2 u =>
     let u' := match Nat.eq_dec x1 x', Nat.eq_dec x2 x' with | left _, left _ | left _, right _ | right _, left _ => u | right _, right _ => term_sub u x' v' end in
     term_PatP (term_sub t x' v') m x1 x2 u'
-  | term_PatE t m n x u => 
+  | term_PatE t m n x u =>
     let u' := match Nat.eq_dec x x' with | left _ => u | right _ => term_sub u x' v' end in
     term_PatE (term_sub t x' v') m n x u'
   | term_Map t x t' =>
@@ -589,23 +591,46 @@ Proof.
   - apply le_S. assumption.
 Qed.
 
+(* Defined separately from `ctx_hdn_shift` for two reasons: this
+   avoids Program adding a bunch of equality, so the function is
+   cleaner. And it makes it possible to state the
+   `preshift_binding_type_eq` lemma. *)
+Definition preshift (H : hdns) (h' : hdn) (n : name): name :=
+  match n with
+  | name_Var x => name_Var x
+  | name_DH h => name_DH (
+                    match (ge_dec h h') with
+                    | left _ => match (HdnsM.mem (h-h') H) with
+                               | true => h - h'
+                               | false => h
+                               end
+                    | right _ => match (HdnsM.mem h H) with
+                                | true => h + h'
+                                | false => h
+                                end
+                    end
+                  )
+  end.
+
+Lemma preshift_binding_type_eq : forall H h'
+  , binding_type_of = fun n => binding_type_of (preshift H h' n).
+Proof.
+  intros *.
+  apply functional_extensionality.
+  intros [xx|xh].
+  all: reflexivity.
+Defined.
+
+Definition post_process H h' n : binding_type_of (preshift H h' n) -> binding_type_of n :=
+  match n with
+  | name_Var _ => fun b => b
+  | name_DH _ => fun b => b
+  end.
+
 #[program]
-Definition ctx_hdn_shift (G : ctx) (H : hdns) (h' : hdn) :=
-  precomp (fun n => match n with
-      | name_Var x => name_Var x
-      | name_DH h => name_DH (
-          match (ge_dec h h') with
-            | left _ => match (HdnsM.mem (h-h') H) with
-              | true => h - h'
-              | false => h
-              end
-            | right _ => match (HdnsM.mem h H) with
-              | true => h + h'
-              | false => h
-              end
-          end
-        )
-      end)
+Definition ctx_hdn_shift (G : ctx) (H : hdns) (h' : hdn) : ctx :=
+  map (post_process H h') (
+  precomp (preshift H h')
     (
       fun n => match n with
       | name_Var x => cons (name_Var x) nil
@@ -618,9 +643,9 @@ Definition ctx_hdn_shift (G : ctx) (H : hdns) (h' : hdn) :=
           | true, left _, false => cons (name_DH h) (cons (name_DH (h+h')) nil)
           end
       end
-    ) G.
+    ) G).
 Next Obligation.
-  destruct w; unfold List.In.
+  destruct w; unfold List.In, preshift.
   - rewrite <- or_false_equiv. reflexivity.
   - destruct (ge_dec h h') eqn:egehhp.
     * destruct (HdnsM.mem (h-h') H) eqn:ememhmhp.
@@ -673,7 +698,7 @@ Inductive TyR_val : ctx -> val -> type -> Prop :=    (* defn TyR_val *)
  | TyR_val_D : forall (G:ctx) (h:hdn) (T:type) (n:mode)
      (CompatGh: ctx_CompatibleDH G h (tyb_Dest  (Some (pair   Lin     (Fin 0)  ))  T n) ),
      TyR_val G (val_D h) (type_D T n)
- | TyR_val_U : 
+ | TyR_val_U :
      TyR_val  ctx_empty  val_U type_U
  | TyR_val_F : forall (D:ctx) (x:var) (m:mode) (u:term) (T U:type)
      (Validm: mode_IsValid m )
@@ -940,7 +965,7 @@ Inductive Sem_eterm : ectxs -> term -> ectxs -> term -> Prop :=    (* defn Sem_e
  | Sem_eterm_AppUnfoc2 : forall (C:ectxs) (v v':val),
      Sem_eterm   (cons   (ectx_AppFoc2 v)    C )   (term_Val v') C (term_App (term_Val v) (term_Val v'))
  | Sem_eterm_AppRed : forall (C:ectxs) (v:val) (x:var) (m:mode) (u:term),
-     Sem_eterm C (term_App (term_Val v) (term_Val  (val_F x m u) )) C  (term_sub  u   x   v ) 
+     Sem_eterm C (term_App (term_Val v) (term_Val  (val_F x m u) )) C  (term_sub  u   x   v )
  | Sem_eterm_PatUFoc : forall (C:ectxs) (t u:term)
      (NotValt: term_NotVal t ),
      Sem_eterm C (term_PatU t u)   (cons   (ectx_PatUFoc u)    C )   t
@@ -954,23 +979,23 @@ Inductive Sem_eterm : ectxs -> term -> ectxs -> term -> Prop :=    (* defn Sem_e
  | Sem_eterm_PatSUnfoc : forall (C:ectxs) (m:mode) (x1:var) (u1:term) (x2:var) (u2:term) (v:val),
      Sem_eterm   (cons   (ectx_PatSFoc m x1 u1 x2 u2)    C )   (term_Val v) C (term_PatS (term_Val v) m x1 u1 x2 u2)
  | Sem_eterm_PatLRed : forall (C:ectxs) (v1:val) (m:mode) (x1:var) (u1:term) (x2:var) (u2:term),
-     Sem_eterm C (term_PatS (term_Val  (val_L v1) ) m x1 u1 x2 u2) C  (term_sub  u1   x1   v1 ) 
+     Sem_eterm C (term_PatS (term_Val  (val_L v1) ) m x1 u1 x2 u2) C  (term_sub  u1   x1   v1 )
  | Sem_eterm_PatRRed : forall (C:ectxs) (v2:val) (m:mode) (x1:var) (u1:term) (x2:var) (u2:term),
-     Sem_eterm C (term_PatS (term_Val  (val_R v2) ) m x1 u1 x2 u2) C  (term_sub  u2   x2   v2 ) 
+     Sem_eterm C (term_PatS (term_Val  (val_R v2) ) m x1 u1 x2 u2) C  (term_sub  u2   x2   v2 )
  | Sem_eterm_PatPFoc : forall (C:ectxs) (t:term) (m:mode) (x1 x2:var) (u:term)
      (NotValt: term_NotVal t ),
      Sem_eterm C (term_PatP t m x1 x2 u)   (cons   (ectx_PatPFoc m x1 x2 u)    C )   t
  | Sem_eterm_PatPUnfoc : forall (C:ectxs) (m:mode) (x1 x2:var) (u:term) (v:val),
      Sem_eterm   (cons   (ectx_PatPFoc m x1 x2 u)    C )   (term_Val v) C (term_PatP (term_Val v) m x1 x2 u)
  | Sem_eterm_PatPRed : forall (C:ectxs) (v1 v2:val) (m:mode) (x1 x2:var) (u:term),
-     Sem_eterm C (term_PatP (term_Val (val_P v1 v2)) m x1 x2 u) C  (term_sub   (term_sub  u   x1   v1 )    x2   v2 ) 
+     Sem_eterm C (term_PatP (term_Val (val_P v1 v2)) m x1 x2 u) C  (term_sub   (term_sub  u   x1   v1 )    x2   v2 )
  | Sem_eterm_PatEFoc : forall (C:ectxs) (t:term) (m n:mode) (x:var) (u:term)
      (NotValt: term_NotVal t ),
      Sem_eterm C (term_PatE t m n x u)   (cons   (ectx_PatEFoc m n x u)    C )   t
  | Sem_eterm_PatEUnfoc : forall (C:ectxs) (m n:mode) (x:var) (u:term) (v:val),
      Sem_eterm   (cons   (ectx_PatEFoc m n x u)    C )   (term_Val v) C (term_PatE (term_Val v) m n x u)
  | Sem_eterm_PatERed : forall (C:ectxs) (n:mode) (v':val) (m:mode) (x:var) (u:term),
-     Sem_eterm C (term_PatE (term_Val (val_E n v')) m n x u) C  (term_sub  u   x   v' ) 
+     Sem_eterm C (term_PatE (term_Val (val_E n v')) m n x u) C  (term_sub  u   x   v' )
  | Sem_eterm_MapFoc : forall (C:ectxs) (t:term) (x:var) (t':term)
      (NotValt: term_NotVal t ),
      Sem_eterm C (term_Map t x t')   (cons   (ectx_MapFoc x t')    C )   t
@@ -978,7 +1003,7 @@ Inductive Sem_eterm : ectxs -> term -> ectxs -> term -> Prop :=    (* defn Sem_e
      Sem_eterm   (cons   (ectx_MapFoc x t')    C )   (term_Val v) C (term_Map (term_Val v) x t')
  | Sem_eterm_MapRedAOpenFoc : forall (C:ectxs) (H:hdns) (v2 v1:val) (x:var) (t':term) (h':hdn)
      (hpMaxC: h' =  (  (hdns_max   (hdns_from_ectxs  C )  )   +   1  )  ),
-     Sem_eterm C (term_Map (term_Val (val_A H v2 v1)) x t')   (cons   (ectx_AOpenFoc  (hdns_shift  H   h' )   (val_hdn_shift  v2   H   h' ) )    C )    (term_sub  t'   x    (val_hdn_shift  v1   H   h' )  ) 
+     Sem_eterm C (term_Map (term_Val (val_A H v2 v1)) x t')   (cons   (ectx_AOpenFoc  (hdns_shift  H   h' )   (val_hdn_shift  v2   H   h' ) )    C )    (term_sub  t'   x    (val_hdn_shift  v1   H   h' )  )
  | Sem_eterm_AOpenUnfoc : forall (C:ectxs) (H:hdns) (v2 v1:val),
      Sem_eterm   (cons  (ectx_AOpenFoc H v2)   C )   (term_Val v1) C (term_Val (val_A H v2 v1))
  | Sem_eterm_AllocRed : forall (C:ectxs),
@@ -1056,5 +1081,3 @@ Inductive Sem_eterm : ectxs -> term -> ectxs -> term -> Prop :=    (* defn Sem_e
  | Sem_eterm_FillCRed : forall (C:ectxs) (h:hdn) (H:hdns) (v2 v1:val) (h':hdn)
      (hpMaxCh: h' =  (  (hdns_max   (HdnsM.union   (hdns_from_ectxs  C )     (hdns_from_list  (cons h nil) )  )  )   +   1  )  ),
      Sem_eterm C (term_FillC (term_Val (val_D h)) (term_Val (val_A H v2 v1)))  (ectxs_fill  C   h     (hdns_shift  H   h' )      (val_hdn_shift  v2   H   h' )  )  (term_Val  (val_hdn_shift  v1   H   h' ) ).
-
-
